Multiple minor changes including a fix to a bug found by Guodong Li.

examples/mc-logic/set_sepLib.sig
@@ -24,6 +24,7 @@ sig
     val MOVE_STAR_CONV      : term frag list -> term frag list -> conv
     val MOVE_STAR_RULE      : term frag list -> term frag list -> rule
 
+    val MOVE_OUT_AUX_CONV        : (term -> bool) -> conv
     val MOVE_OUT_TERM_CONV       : term -> conv
     val MOVE_OUT_CONV            : term frag list -> conv
     val MOVE_OUT_LIST_TERM_CONV  : term list -> conv
